thys/Applicative_Lifting/Stream_Algebra.thy
@@ -20,25 +20,25 @@ end
 
 instantiation stream :: (plus) plus begin
 interpretation applicative_syntax .
-definition [applicative_unfold]: "x + y = pure op + \<diamond> x \<diamond> (y :: 'a stream)"
+definition [applicative_unfold]: "x + y = pure op + \<diamondop> x \<diamondop> (y :: 'a stream)"
 instance ..
 end
 
 instantiation stream :: (minus) minus begin
 interpretation applicative_syntax .
-definition [applicative_unfold]: "x - y = pure op - \<diamond> x \<diamond> (y :: 'a stream)"
+definition [applicative_unfold]: "x - y = pure op - \<diamondop> x \<diamondop> (y :: 'a stream)"
 instance ..
 end
 
 instantiation stream :: (uminus) uminus begin
 interpretation applicative_syntax .
-definition [applicative_unfold stream]: "uminus = (op \<diamond> (pure uminus) :: 'a stream \<Rightarrow> 'a stream)"
+definition [applicative_unfold stream]: "uminus = (op \<diamondop> (pure uminus) :: 'a stream \<Rightarrow> 'a stream)"
 instance ..
 end
 
 instantiation stream :: (times) times begin
 interpretation applicative_syntax .
-definition [applicative_unfold]: "x * y = pure op * \<diamond> x \<diamond> (y :: 'a stream)"
+definition [applicative_unfold]: "x * y = pure op * \<diamondop> x \<diamondop> (y :: 'a stream)"
 instance ..
 end
 
@@ -46,8 +46,8 @@ instance stream :: (Rings.dvd) Rings.dvd ..
 
 instantiation stream :: ("Divides.div") "Divides.div" begin
 interpretation applicative_syntax .
-definition [applicative_unfold]: "x div y = pure op div \<diamond> x \<diamond> (y :: 'a stream)"
-definition [applicative_unfold]: "x mod y = pure op mod \<diamond> x \<diamond> (y :: 'a stream)"
+definition [applicative_unfold]: "x div y = pure op div \<diamondop> x \<diamondop> (y :: 'a stream)"
+definition [applicative_unfold]: "x mod y = pure op mod \<diamondop> x \<diamondop> (y :: 'a stream)"
 instance ..
 end
 
